denning-sacco-central-auth/DS.Clock.fst
@@ -1,12 +1,16 @@
 module DS.Clock
 
 
+open GlobalRuntimeLib
+open LabeledCryptoAPI
+
+
 (* Internal clock type *)
 let clock_ = (counter:nat * timestamp)
 
 (* Adds 'd' to the clocks counter *)
-let clock_add (clock:clock_) (d:nat) : clock_ =
-  let (counter, ts) = clock in (counter + d, ts)
+let clock_add (c:clock_) (d:nat) : clock_ =
+  let (counter, ts) = c in (counter + d, ts)
 
 
 (* Interface implementation *)
@@ -17,9 +21,17 @@ let clock = clock_
 let clock_get clock =
   let (counter, _) = clock in counter
 
-let clock_new () = let ts = global_timestamp () in (0, ts)
+let clock_new #pr p =
+  let ts = global_timestamp () in
+  let _ = L.send #pr #ts p p (nat_to_bytes #pr.global_usage #ts 0 ts) in
+  (|(0, ts),ts|)
 
-let clock_lte ts base_cnt cmp =
-  let (cnt_cmp, ts_cmp) = cmp in
-  if ts_cmp = ts then Success (cnt_cmp <= base_cnt)
+let att_clock_new () =
+  let ts = A.global_timestamp () in
+  let _ = A.send #ts "*" "*" (A.pub_bytes_later 0 ts (A.nat_to_pub_bytes 0 ts)) in
+  (|(0, ts),ts|)
+
+let clock_lte ts max_delay c =
+  let (cnt_c, ts_c) = c in
+  if ts_c = ts then Success (cnt_c <= max_delay)
   else Error "[clock_lte] Timestamps do not match"
