denning-sacco-central-auth/DS.Clock.fsti
@@ -2,8 +2,11 @@ module DS.Clock
 
 
 open CryptoEffect
-open GlobalRuntimeLib
 open SecrecyLabels
+open LabeledRuntimeAPI
+
+module L = LabeledPKI
+module A = AttackerAPI
 
 
 /// Clock measuring number of sends and receives in a specific Denning-Sacco
@@ -11,22 +14,37 @@ open SecrecyLabels
 val clock:Type0
 
 /// Get the value of the clocks counter
-val clock_get: clock:clock -> nat
+val clock_get: c:clock -> nat
 
 /// Outputs a new clock with the current timestamp and a fresh counter
-val clock_new: unit -> Crypto clock
+val clock_new: #pr:preds -> principal ->
+  LCrypto (c_new:clock & ts:timestamp) (L.pki pr)
+  (requires (fun t0 -> True))
+  (ensures (fun t0 (|c_new,ts|) t1 ->
+    trace_len t1 == (trace_len t0) + 1  /\
+    clock_get c_new == 0 /\
+    ts == trace_len t0))
+
+/// Outputs a new clock with the current timestamp and a fresh counter
+val att_clock_new: unit ->
+  Crypto (c_new:clock & ts:timestamp)
   (requires (fun t0 -> True))
   (ensures (fun t0 r t1 ->
     match r with
-    | Success clock -> t1 == t0 /\ clock_get clock == 0
-    | _ -> False
+    | Success (|c_new,ts|) ->
+      A.attacker_modifies_trace t0 t1 /\
+      trace_len t1 == (trace_len t0) + 1 /\
+      later_than (trace_len t1) (trace_len t0) /\
+      clock_get c_new == 0 /\
+      ts == trace_len t0
+    | Error _ -> t0 == t1
   ))
 
-/// Tests whether 'base_cnt' is less than or equal to the value of the counter of 'cmp'.
+/// Tests whether 'max_delay' is less than or equal to the value of the counter of 'c'.
 /// Outputs an error if the timestamp does not match with the clocks timestamp.
-val clock_lte: ts:timestamp -> base_cnt:nat -> cmp:clock -> r:(result bool)
+val clock_lte: ts:timestamp -> max_delay:nat -> c:clock -> r:(result bool)
   {
     match r with
-    | Success true -> clock_get cmp <= base_cnt
+    | Success true -> clock_get c <= max_delay
     | _ -> True
   }
